\documentclass{article}
\usepackage{amsmath}
\usepackage{amssymb}

\begin{document}

\[
\int \sqrt{x^2+1}\,dx
\]

\textbf{Substitution ($u=a\tan\theta$ with $a=1,\ u=x$):} \quad $x=\tan\theta,\quad dx=\sec^2\theta\,d\theta,\quad \sqrt{x^2+1}=\sqrt{\tan^2\theta+1}=\sec\theta$.

\[
\int \sqrt{x^2+1}\,dx = \int \sec\theta \cdot \sec^2\theta\,d\theta = \int \sec^3\theta\,d\theta
\]

\textbf{Let $I = \int \sec^3\theta\,d\theta$. Integration by parts:} $\displaystyle I = \int \sec\theta \cdot \sec^2\theta\,d\theta$, take $f = \sec\theta,\ g' = \sec^2\theta \Rightarrow f' = \sec\theta\tan\theta,\ g = \tan\theta$.

\[
I = \sec\theta\tan\theta - \int (\sec\theta\tan\theta)\tan\theta\,d\theta
\]

\textbf{Identity:} $\tan^2\theta = \sec^2\theta - 1$.

\[
I = \sec\theta\tan\theta - \int \sec\theta(\sec^2\theta-1)\,d\theta
= \sec\theta\tan\theta - \int \sec^3\theta\,d\theta + \int \sec\theta\,d\theta
\]

\[
2I = \sec\theta\tan\theta + \int \sec\theta\,d\theta
\]

\textbf{Formula:} $\displaystyle \int \sec\theta\,d\theta = \ln|\sec\theta+\tan\theta| + C$.

\[
I = \frac{1}{2}\sec\theta\tan\theta + \frac{1}{2}\ln|\sec\theta+\tan\theta| + C
\]

\textbf{Back-substitution:} $\sec\theta = \sqrt{1+x^2},\ \tan\theta = x$.

\[
\boxed{
  \int \sqrt{x^2+1}\,dx = \frac{1}{2}\,x\sqrt{x^2+1} + \frac{1}{2}\,\ln\!\left|x+\sqrt{x^2+1}\right| + C
}
\]

\end{document}